{
  "@context": {
    "schema": "http://schema.org/",
    "rdf": "http://www.w3.org/1999/02/22-rdf-syntax-ns#",
    "rdfs": "http://www.w3.org/2000/01/rdf-schema#",
    "bioschemas": "https://discovery.biothings.io/view/bioschemas/",
    "niaid": "https://discovery.biothings.io/view/niaid/",
    "nde": "https://discovery.biothings.io/view/nde/"
  },
  "@graph": [{
      "@id": "nde:Dataset",
      "@type": "rdfs:Class",
      "rdfs:comment": "Datasets contained in the NIAID Data Ecosystem. The NIAID Data Ecosystem is a secure environment to find, access and analyze immune-mediated and infectious disease data and computational tools to speed the development of diagnostics, therapeutics, and vaccines. The NIAID Data Ecosystem Discovery Portal harvests metadata from dataset repository and harmonizes them to this schema to enable easy cross-platform dataset searching and filtering.",
      "rdfs:label": "Dataset",
      "rdfs:subClassOf": {
        "@id": "niaid:Dataset"
      },
      "$validation": {
        "$schema": "http://json-schema.org/draft-07/schema#",
        "type": "object",
        "properties": {
          "doi": {
            "description": "Digital object identifier (DOI) for the Dataset",
            "owl:cardinality": "one",
            "type": "string"
          },
          "description": {
            "description": "A description of the item.",
            "owl:cardinality": "one",
            "type": "string"
          }
        },
        "required": [
          "description"
        ],
        "recommended": [
          "doi"
        ]
      }
    },
    {
      "@id": "nde:doi",
      "@type": "rdf:Property",
      "rdfs:comment": "Digital Object Identifier (DOI) for the Dataset. Note: the DOI should be a permanent identifier for the Dataset itself, not any publications associated with the Dataset.",
      "rdfs:label": "doi",
      "schema:domainIncludes": [{
          "@id": "nde:Dataset"
        },
        {
          "@id": "nde:ComputationalTool"
        }
      ],
      "schema:rangeIncludes": [{
        "@id": "schema:Text"
      }]
    },
    {
      "@id": "nde:ComputationalTool",
      "@type": "rdfs:Class",
      "rdfs:comment": "ComputationalTools (software, workflows, computational tools, code) contained in the NIAID Data Ecosystem. The NIAID Data Ecosystem is a secure environment to find, access and analyze immune-mediated and infectious disease data and computational tools to speed the development of diagnostics, therapeutics, and vaccines. The NIAID Data Ecosystem Discovery Portal harvests metadata from dataset repository and harmonizes them to this schema to enable easy cross-platform dataset searching and filtering.",
      "rdfs:label": "ComputationalTool",
      "rdfs:subClassOf": {
        "@id": "niaid:ComputationalTool"
      },
      "$validation": {
        "$schema": "http://json-schema.org/draft-07/schema#",
        "type": "object",
        "properties": {
          "doi": {
            "description": "Digital object identifier (DOI) for the ComputationalTool",
            "owl:cardinality": "one",
            "type": "string"
          },
          "description": {
            "description": "A description of the item.",
            "owl:cardinality": "one",
            "type": "string"
          }
        },
        "required": [
          "description"
        ],
        "recommended": [
          "doi"
        ],
        "definitions": {}
      }
    }
  ]
}
